examples/riscv/chacha/chacha_symb_transf_quarterroundScript.sml
@@ -19,17 +19,17 @@ val _ = new_theory "chacha_symb_transf_quarterround";
 val bspec_cont_thm =
  bir_symb_transfer_thm
   bir_chacha_prog_def
-  chacha_quarterround_init_addr_def chacha_quarterround_end_addr_def
-  bspec_chacha_quarterround_pre_def bspec_chacha_quarterround_post_def
+  chacha_line_init_addr_def chacha_line_end_addr_def
+  bspec_chacha_line_pre_def bspec_chacha_line_post_def
   chacha_birenvtyl_def chacha_prog_vars_list_def
-  chacha_quarterround_symb_analysis_thm NONE chacha_prog_vars_thm;
+  chacha_line_symb_analysis_thm NONE chacha_prog_vars_thm;
 
-val init_addr_tm = (snd o dest_eq o concl) chacha_quarterround_init_addr_def;
-val end_addr_tm = (snd o dest_eq o concl) chacha_quarterround_end_addr_def;
-val bspec_pre_tm = (lhs o snd o strip_forall o concl) bspec_chacha_quarterround_pre_def;
-val bspec_post_tm = (lhs o snd o strip_forall o concl) bspec_chacha_quarterround_post_def;
+val init_addr_tm = (snd o dest_eq o concl) chacha_line_init_addr_def;
+val end_addr_tm = (snd o dest_eq o concl) chacha_line_end_addr_def;
+val bspec_pre_tm = (lhs o snd o strip_forall o concl) bspec_chacha_line_pre_def;
+val bspec_post_tm = (lhs o snd o strip_forall o concl) bspec_chacha_line_post_def;
 
-Theorem bspec_cont_chacha_quarterround:
+Theorem bspec_cont_chacha_line:
  bir_cont bir_chacha_prog bir_exp_true
   (BL_Address (Imm64 ^init_addr_tm)) {BL_Address (Imm64 ^end_addr_tm)} {}
   ^bspec_pre_tm
@@ -40,22 +40,22 @@ Proof
  rw [bspec_cont_thm]
 QED
 
-(* second quarterround *)
+(* second line *)
 
 val bspec_cont_thm =
  bir_symb_transfer_thm
   bir_chacha_prog_def
-  chacha_other_quarterround_init_addr_def chacha_other_quarterround_end_addr_def
-  bspec_chacha_quarterround_pre_other_def bspec_chacha_quarterround_post_other_def
+  chacha_other_line_init_addr_def chacha_other_line_end_addr_def
+  bspec_chacha_line_pre_other_def bspec_chacha_line_post_other_def
   chacha_birenvtyl_def chacha_prog_vars_list_def
-  chacha_other_quarterround_symb_analysis_thm NONE chacha_prog_vars_thm;
+  chacha_other_line_symb_analysis_thm NONE chacha_prog_vars_thm;
 
-val init_addr_tm = (snd o dest_eq o concl) chacha_other_quarterround_init_addr_def;
-val end_addr_tm = (snd o dest_eq o concl) chacha_other_quarterround_end_addr_def;
-val bspec_pre_tm = (lhs o snd o strip_forall o concl) bspec_chacha_quarterround_pre_other_def;
-val bspec_post_tm = (lhs o snd o strip_forall o concl) bspec_chacha_quarterround_post_other_def;
+val init_addr_tm = (snd o dest_eq o concl) chacha_other_line_init_addr_def;
+val end_addr_tm = (snd o dest_eq o concl) chacha_other_line_end_addr_def;
+val bspec_pre_tm = (lhs o snd o strip_forall o concl) bspec_chacha_line_pre_other_def;
+val bspec_post_tm = (lhs o snd o strip_forall o concl) bspec_chacha_line_post_other_def;
 
-Theorem bspec_cont_chacha_other_quarterround:
+Theorem bspec_cont_chacha_other_line:
  bir_cont bir_chacha_prog bir_exp_true
   (BL_Address (Imm64 ^init_addr_tm)) {BL_Address (Imm64 ^end_addr_tm)} {}
   ^bspec_pre_tm
